theories/Prelude/Notations.v
@@ -1,1 +1,9 @@
 Require Import LoL.Prelude.Prelude.
+
+Reserved Infix ">>=" (left associativity, at level 90).
+
+Module MonadNotations.
+
+Infix ">>=" := bind.
+
+End MonadNotations.
